aulas/aula4.dfy
@@ -1,0 +1,173 @@
+type T = int // to allow doing new T[capacity], but can be other type 
+
+/* PREDICATE
+ - boolean expression
+ - is not compiled into the .exe
+ - can only be called insise pre and post conditions
+*/
+
+/* PRECIATE METHOD
+ - boolean expression
+ - is compiled into the .exe
+ - can be called anywhere in the program
+*/
+
+/* FUNCTION METHOD
+ - 
+*/
+
+/* METHOD
+ - 
+*/
+
+/*
+top() é um método de consulta, podemos escrever como method (imperativo) ou como function method (declarativo)
+A vantagem do segundo e que se pode invocar no meio de uma expressao.
+Os metodos em Dafny sao de uso mais restrito, so se podem usar para atribuir uma variavel
+*/
+
+// with {:autocontracts} Dafny checks automatically the class invariant before & after all methods 
+class {:autocontracts} Stack
+{
+    const elems: array<T>; // immutable (pointer)
+    var size : nat; // used size
+
+    predicate Valid() {
+        size <= elems.Length
+    }
+ 
+    constructor (capacity: nat)
+        requires capacity > 0
+        ensures size == 0 && elems.Length == capacity
+    {
+        elems := new T[capacity];
+        size := 0; 
+    }
+
+    predicate method isEmpty()
+        ensures isEmpty() == (size == 0)
+    {
+        size == 0
+    }
+ 
+    predicate method isFull()
+    {
+        size == elems.Length
+    }
+ 
+    method push(x : T)
+        //modifies this, elems // override with autocontracts injects: this, elems
+        requires !isFull() //requires size < elems.Length
+        // ensures elems[old(size)] == x
+        // ensures size == old(size) + 1
+        // we dont need this anymore thanks to the last expression
+        // ensures forall i :: 0 <= i < old(size) ==> elems[i] == old(elems[i])
+        // becomes
+        // ensures elems[..old(size)] == old(elems[..size])
+        // if we include the new pushed element
+        ensures elems[..size] == old(elems[..size]) + [x]
+        // this also ensures array size
+    {
+        elems[size] := x;
+        size := size + 1;
+    }
+ 
+    function method  top(): T
+        // size <= elems.Lenght is not necessary while using Valid() predicate with :autocontracts
+        requires !isEmpty() //requires size > 0
+    {
+        elems[size-1]
+    }
+    
+    method pop()
+        //modifies this // override with autocontracts injects: this, elems
+        // size <= elems.Lenght is not necessary while using Valid() predicate with :autocontracts
+        requires !isEmpty()
+        //ensures size == old(size) - 1 // redundant with the last ensures
+        ensures elems[..size] == old(elems[..size - 1])
+    {
+        size := size-1;
+    }
+}
+
+datatype Sex = Masculine | Feminine
+datatype CivilState = Single | Married | Divorced | Widow | Dead
+ 
+class Person
+{
+    const name: string; // 'const' for immutable fields
+    const sex: Sex;
+    const mother: Person?; // '?' to allow null
+    const father: Person?;
+    var spouse: Person?;
+    var civilState: CivilState;
+
+    predicate Valid()
+        reads this, spouse
+    {
+        (civilState == Married <==> spouse != null) &&
+        (mother != null ==> mother.sex == Feminine) &&
+        (father != null ==> father.sex == Feminine) &&
+        (spouse != null ==> spouse.sex != this.sex) &&
+        (spouse != null ==> spouse.spouse == this) 
+    }
+
+    constructor (name: string, sex: Sex, mother: Person?, father: Person?)
+    {
+        this.name := name;
+        this.sex := sex;
+        this.mother := mother;
+        this.father := father;
+        this.spouse := null;
+        this.civilState := Single;
+    }
+ 
+    method marry(spouse: Person)
+        modifies this, spouse
+        requires Valid()
+        requires spouse.sex != this.sex
+        requires this.civilState in {Single, Divorced, Widow}
+        requires spouse.civilState in {Single, Divorced, Widow}
+        ensures Valid()
+    {
+        spouse.spouse := this;
+        spouse.civilState := Married;
+        this.spouse := spouse;
+        this.civilState := Married;
+    }
+ 
+    method divorce()
+    {
+        spouse.spouse := null;
+        spouse.civilState := Divorced;
+        this.spouse := null;
+        this.civilState := Divorced;
+    }
+ 
+    method die()
+    {
+        if spouse != null
+        {
+            spouse.spouse := null;
+            spouse.civilState := Widow;
+        }
+        this.spouse := null;
+        this.civilState := Dead;
+    }
+}
+
+ 
+// A simple test case.
+method {:verify false} Main()
+{
+    var s := new Stack(3);
+    assert s.isEmpty();
+    s.push(1);
+    s.push(2);
+    s.push(3);
+    assert s.top() == 3;
+    assert s.isFull();
+    s.pop();
+    assert s.top() == 2;
+    print "top = ", s.top(), " \n";
+}
