aulas/aula5.dfy
@@ -1,0 +1,86 @@
+type T = int // for demo purposes, but could be another type
+ 
+class {:autocontracts} Deque {
+    // (Private) concrete state variables 
+    const list: array<T>; // circular array, from list[start] (front) to 
+                             list[(start+size-1) % list.Length] (back) 
+    var start : nat; 
+    var size : nat;
+ 
+    constructor (capacity: nat) {
+        list := new T[capacity];
+        start := 0;
+        size := 0;
+    }
+ 
+    predicate method isEmpty() {
+        size == 0
+    }
+    
+    predicate method isFull() {
+        size == list.Length
+    }
+ 
+    function method front() : T {
+        list[start]
+    }
+ 
+    function method back() : T {
+        list[(start + size - 1) % list.Length] 
+    }
+    
+    method push_back(x : T) {
+        list[(start + size) % list.Length] := x;
+        size := size + 1;
+    }
+ 
+    method pop_back() {
+        size := size - 1;
+    }
+ 
+    method push_front(x : T) {
+        if start > 0 {
+            start := start - 1;
+        }
+        else {
+            start := list.Length - 1;
+        }
+        list[start] := x;
+        size := size + 1;
+    }    
+ 
+    method pop_front() {
+        if start + 1 < list.Length {
+            start := start + 1;
+        }
+        else {
+            start := 0;
+        }
+        size := size - 1;
+    } 
+}
+ 
+// A simple test scenario.
+method testDeque()
+{
+    var q := new Deque(3);
+    assert q.isEmpty();
+    q.push_front(1);
+    assert q.front() == 1;
+    assert q.back() == 1;
+    q.push_front(2);
+    assert q.front() == 2;
+    assert q.back() == 1;
+    q.push_back(3);
+    assert q.front() == 2;
+    assert q.back() == 3;
+    assert q.isFull();
+    q.pop_back();
+    assert q.front() == 2;
+    assert q.back() == 1;
+    q.pop_front();
+    assert q.front() == 1;
+    assert q.back() == 1;
+    q.pop_front();
+    assert q.isEmpty();
+}
